Forgot orderedBItvec

TransVal/orderedBitvec.v
@@ -4,11 +4,6 @@ Require Import Util List OrderedType bitvec.
 Inductive ltBit :bit-> bit -> Prop :=
 |ltBitO :  ltBit O I.
 
-(** Equality predicate for bits *)
-Inductive eqBit : bit->bit -> Prop :=
-|eqBitO :  eqBit O O
-|eqBitI :  eqBit I I.
-
 Definition bitCmp (b1:bit) (b2:bit) :=
 match b1,b2 with
 |O, O => Eq
@@ -17,81 +12,44 @@ match b1,b2 with
 | I, I => Eq
 end.
 
-Lemma bitEq_reflexive :
-Reflexive eqBit.
-
-Proof.
-unfold Reflexive. intros. destruct x; econstructor.
-Qed.
-
-Lemma bitEq_symm:
-Symmetric eqBit.
-
-Proof.
-unfold Symmetric. intros. general induction H; econstructor.
-Qed.
-
-Lemma bitEq_trans:
-Transitive eqBit.
-
-Proof.
-unfold Transitive. intros. general induction H.
-- assumption.
-- assumption.
-Qed.
-
-Instance equiv_eqbit: Equivalence eqBit.
-econstructor.
-- exact bitEq_reflexive.
-- exact bitEq_symm.
-- exact bitEq_trans.
-Defined.
-
-Lemma ltBit_trans:
+Instance ltBit_trans:
 Transitive ltBit.
 
-Proof.
 unfold Transitive. intros. general induction H.
 - general induction H0.
-Qed.
+Defined.
 
-Lemma ltBit_irrefl:
+Instance ltBit_irrefl:
 Irreflexive ltBit.
 
-Proof.
 hnf; intros. unfold RelationClasses.complement. induction x.
 - intros. inversion H.
 - intros. inversion H.
-Qed.
-
-Instance  rewrite_eqBit: forall x, Proper (eqBit ==> flip impl) (ltBit x).
-unfold Proper, respectful. intros.  unfold flip.  unfold impl.  intros.  general induction H0.
-- general induction H. econstructor.
 Defined.
 
-Instance lt_eq_bit_strict: OrderedType.StrictOrder ltBit eqBit.
+Instance  rewrite_eqBit: forall x, Proper (eq ==> flip impl) (ltBit x).
+unfold Proper, respectful. intros.  unfold flip.  unfold impl.  intros.  general induction H0.
+-  econstructor.
+Defined.
+
+Instance lt_eq_bit_strict: OrderedType.StrictOrder ltBit eq.
 econstructor.
 - exact ltBit_trans.
 - intros. intro. apply (ltBit_irrefl x). rewrite <- H0 in H. assumption.
 Defined.
 
 Instance OrderedType_bit : OrderedType bit :=
-{ _eq := eqBit;
+{ _eq := eq;
   _lt := ltBit;
   _cmp := bitCmp}.
 intros. general induction x; destruct y; simpl; try now (econstructor; eauto using ltBit).
-Qed.
+Defined.
 
 (** Inductive lt predicate for bitvectors **)
 Inductive ltBitvec : bitvec -> bitvec -> Prop :=
 |ltBitvecNil a b: ltBitvec nil (a::b)
 |ltBitvecCons a b c d : _lt a c ->  ltBitvec (a::b) (c::d)
 |ltBitvecEq a b c d: _eq a c -> ltBitvec b d -> ltBitvec (a::b) (c::d).
-
-(** Equality predicate for bitvectors **)
-Inductive eqBitvec:  bitvec -> bitvec -> Prop :=
-|eqNil: eqBitvec nil nil
-|eqCons a b c d: _eq a c -> eqBitvec b d -> eqBitvec (a::b) (c::d).
 
 Fixpoint bvCmp  (a:bitvec) ( b:bitvec) :=
 match a,b with
@@ -115,51 +73,9 @@ end.
                                     end
 end.*)
 
-Lemma bitvecEq_reflexive :
-Reflexive eqBitvec.
-
-Proof.
-unfold Reflexive. intros. general induction x.
-- econstructor.
--  econstructor.
-   * eauto.
-   * assumption.
-Qed. 
-
-Lemma bitvecEq_symm:
-Symmetric eqBitvec.
-
-Proof.
-unfold Symmetric. intros. general induction H.
-- econstructor.
-- econstructor.  
-  * eauto.
-  * assumption.
-Qed.
-
-Lemma bitvecEq_trans:
-Transitive eqBitvec.
-
-Proof.
-unfold Transitive. intros. general induction H.
-- assumption.
--  general induction H1.
-   + econstructor. 
-     *  apply transitivity with c0; eauto.
-     * eapply (IHeqBitvec0). assumption.
-Qed.
-
-Instance equiv_eqbitvec : Equivalence eqBitvec.
-econstructor.
-- exact bitvecEq_reflexive.
-- exact bitvecEq_symm.
-- exact bitvecEq_trans.
-Defined.  
-
-Lemma ltBitvec_trans:
+Instance ltBitvec_trans:
 Transitive ltBitvec.
 
-Proof.
 unfold Transitive. intros. general induction H.
 - general induction H0. 
   + econstructor.
@@ -173,37 +89,35 @@ unfold Transitive. intros. general induction H.
      + econstructor.
        * rewrite H0. assumption.
      + specialize (IHltBitvec0 d). rewrite H in H0. exact (ltBitvecEq a0 b0 c d H0 (IHltBitvec0 H1)).
-Qed.
-
-Lemma ltBitvec_irrefl:
-Irreflexive ltBitvec.
-
-Proof.
-hnf; intros. unfold RelationClasses.complement.  induction x; inversion 1; subst; eauto using StrictOrder_Irreflexive.  
-eapply (StrictOrder_Irreflexive a a H1). intuition.
-Qed.
-
- Instance rewrite_equal_bitvec: forall x, Proper (equiv ==> impl) (ltBitvec x) .
-unfold Proper, respectful. intros.  unfold impl. intros. general induction H0.
-- general induction H. econstructor.
-- general induction H0. econstructor. rewrite H in H1; assumption.
-- general induction H1. rewrite H in H0. exact (ltBitvecEq a0 b0 c d H0 (IHltBitvec d H1)).
 Defined.
 
-Instance lt_eq_strict : OrderedType.StrictOrder ltBitvec eqBitvec.
+Instance ltBitvec_irrefl:
+Irreflexive ltBitvec.
+hnf; intros. unfold RelationClasses.complement.  induction x; inversion 1; subst; eauto using StrictOrder_Irreflexive.  
+eapply (StrictOrder_Irreflexive a a H1). intuition.
+Defined.
+
+ Instance rewrite_equal_bitvec: forall x, Proper (eq ==> impl) (ltBitvec x) .
+unfold Proper, respectful. intros.  unfold impl. intros. general induction H0.
+-  econstructor.
+- econstructor.  assumption.
+- exact (ltBitvecEq a  b c d H H0).
+Defined.
+
+Instance lt_eq_strict : OrderedType.StrictOrder ltBitvec eq.
 econstructor.
 - exact ltBitvec_trans.
 - intros. intro. apply (ltBitvec_irrefl x).   rewrite <-  H0 in H.  assumption. 
 Defined.
 
 Instance OrderedType_bitvec : OrderedType bitvec := 
-  { _eq := eqBitvec;
+  { _eq := eq;
      _lt := ltBitvec;
       _cmp := bvCmp}.
 intros. general induction x; destruct y; simpl; try now (econstructor; eauto using ltBitvec).
 pose proof (_compare_spec a b); destruct (IHx y);
 inv H;  try now (econstructor; eauto using ltBitvec).
--  econstructor.  econstructor; assumption.
+-  econstructor. f_equal. rewrite H2. reflexivity.
 Defined. 
 
 (*
